## Demostración del exámen

$$
n=\frac{Z_0^2pqN}{e^2(N-1)+Z_0^2pq}
$$

Muestra sin remplazamiento

Nota: consideraciones

$$d=|μ-\bar{x}|$$

$$d=\sqrt{(x_2-x_1)^2+(y_2-y_1)^2}$$

$$var(\bar{x})=\frac{\sigma^2}{n}$$

$$var(\bar{x})=\frac{\sigma^2}{n}\cdot \left( \frac{N-n}{N-1} \right)$$

Media poblacional desconocida

$$\sqrt{\sigma_{\bar{x}}^2}=\sqrt{\frac{\sigma_{μ}^2}{n}\cdot \frac{N-n}{N-1}}$$

$$\sigma_{\bar{x}}=\sqrt{\frac{\sigma_{μ}^2}{n}}\cdot \sqrt{\frac{N-n}{N-1}}$$

$$\sigma_{\bar{x}}=\frac{\sigma_{μ}}{\sqrt{n}}\cdot \sqrt{\frac{N-n}{N-1}}$$

$$S.E({\bar{x}})=\frac{\sigma_{μ}}{\sqrt{n}}\cdot \sqrt{\frac{N-n}{N-1}}$$

$$e = S.E({\bar{x}})\cdot Z_0=Z_0\cdot \frac{\sigma_{μ}}{\sqrt{n}}\cdot \sqrt{\frac{N-n}{N-1}}$$

$$e \cdot \sqrt{n} = \sqrt{n} \cdot Z_0\cdot \frac{\sigma_{μ}}{\sqrt{n}}\cdot \sqrt{\frac{N-n}{N-1}}$$

$$e \cdot \sqrt{n} = \cdot Z_0\cdot \sigma_{μ}\cdot \sqrt{\frac{N-n}{N-1}}$$

$$e \cdot \sqrt{n} \cdot \frac{1}{e} =\frac{1}{e} \cdot Z_0\cdot \sigma_{μ}\cdot \sqrt{\frac{N-n}{N-1}}$$

$$\sqrt{n}=\frac{1}{e} \cdot Z_0\cdot \sigma_{μ}\cdot \sqrt{\frac{N-n}{N-1}}$$

$$(\sqrt{n})^2=\left( \frac{1}{e} \cdot Z_0\cdot \sigma_{μ}\cdot \sqrt{\frac{N-n}{N-1}} \right)^2$$

$$(\sqrt{n})^2=\left( \frac{1}{e} \cdot Z_0\cdot \sigma_{μ}\cdot \sqrt{\frac{N-n}{N-1}} \right)^2$$

$$n=Z_0^2\cdot \frac{\sigma_{μ}^2}{e^2} \cdot \frac{N-n}{N-1}$$

$$n=Z_0^2\cdot \frac{\sigma_{μ}^2}{e^2} \left( \frac{N}{N-1} - \frac{n}{N-1} \right)$$

$$n=Z_0^2\cdot \frac{\sigma_{μ}^2}{e^2} \cdot \frac{N}{N-1} - Z_0^2\cdot \frac{\sigma_{μ}^2}{e^2} \cdot \frac{n}{N-1} $$

$$n + Z_0^2\cdot \frac{\sigma_{μ}^2}{e^2} \cdot \frac{n}{N-1} =Z_0^2\cdot \frac{\sigma_{μ}^2}{e^2} \cdot \frac{N}{N-1} $$

$$n \left( 1 + Z_0^2\cdot \frac{\sigma_{μ}^2}{e^2} \cdot \frac{1}{N-1} \right) =Z_0^2\cdot \frac{\sigma_{μ}^2}{e^2} \cdot \frac{N}{N-1} $$

$$n =  Z_0^2\cdot \frac{\sigma_{μ}^2}{e^2} \cdot \frac{N}{N-1} \div \left( 1 + Z_0^2\cdot \frac{\sigma_{μ}^2}{e^2} \cdot \frac{1}{N-1} \right)$$

$$n = \frac{Z_0^2 \cdot \sigma_{μ}^2}{e^2} \cdot \frac{N}{N-1} \div \left( 1 +  \frac{Z_0^2\cdot\sigma_{μ}^2}{e^2} \cdot \frac{1}{N-1} \right)$$

$$n = \frac{Z_0^2 \cdot \sigma_{μ}^2 \cdot N}{e^2 (N -1)} \div \left( 1 +  \frac{Z_0^2\cdot\sigma_{μ}^2 }{e^2 (N-1)} \right)$$

$$n = \frac{Z_0^2 \cdot \sigma_{μ}^2 \cdot N}{e^2 (N -1)} \div \left(   \frac{Z_0^2\cdot\sigma_{μ}^2 + e^2 (N-1) }{e^2 ( N-1)} \right)$$

$$n = \frac{Z_0^2 \cdot \sigma_{μ}^2 \cdot N}{e^2 (N -1)} \cdot \left(   \frac{e^2 ( N-1)}{Z_0^2\cdot\sigma_{μ}^2 + e^2 (N-1)} \right)$$

$$n = \frac{Z_0^2 \cdot \sigma_{μ}^2 \cdot N}{Z_0^2\cdot\sigma_{μ}^2 + e^2 (N-1)}$$

### Proporciones

$$S.E(\bar{p})=\sqrt{\frac{p\cdot q}{n}}\cdot \sqrt{\frac{N-n}{N-1}}$$

$$e = Z_o \cdot S.E(\bar p)$$

$$e = Z_0 \cdot \sqrt{\frac{p\cdot q}{n}}\cdot \sqrt{\frac{N-n}{N-1}}$$

$$e^2 = \left(Z_0 \cdot \sqrt{\frac{p\cdot q}{n}}\cdot \sqrt{\frac{N-n}{N-1}} \right)^2$$

$$e^2 = Z_0^2 \cdot \frac{p\cdot q}{n}\cdot \frac{N-n}{N-1}$$

$$e^2 =  \frac{Z_0^2 \cdot p\cdot q}{n}\cdot \frac{N-n}{N-1}$$

$$e^2 \cdot n = n\cdot \frac{Z_0^2 \cdot p\cdot q}{n}\cdot \frac{N-n}{N-1}$$

$$e^2 \cdot n =   \frac{Z_0^2 \cdot p\cdot q(N-n)}{N-1}$$

$$e^2 \cdot n \cdot \frac{1}{e^2} = \frac{1}{e^2} \cdot \frac{Z_0^2 \cdot p\cdot q(N-n)}{N-1}$$

$$ n = \frac{Z_0^2 \cdot p\cdot q(N-n)}{e^2(N-1)}$$

$$ n \cdot \frac{1}{N-n} = \frac{Z_0^2 \cdot p\cdot q(N-n)}{e^2(N-1)}\cdot \frac{1}{N-n}$$

$$ \frac{n}{N-n} = \frac{Z_0^2 \cdot p\cdot q}{e^2(N-1)}$$

$$ \frac{N-n}{n} = \frac{e^2(N-1)}{Z_0^2 \cdot p\cdot q}$$

$$ \frac{N}{n}-1 = \frac{e^2(N-1)}{Z_0^2 \cdot p\cdot q}$$

$$ \frac{N}{n} = \frac{e^2(N-1)}{Z_0^2 \cdot p\cdot q}+1$$

$$ \frac{N}{n} = \frac{e^2(N-1) + Z_0^2 \cdot p\cdot q}{Z_0^2 \cdot p\cdot q}$$

$$ \frac{n}{N} = \frac{Z_0^2 \cdot p\cdot q}{e^2(N-1) + Z_0^2 \cdot p\cdot q}$$

$$ n = \frac{Z_0^2 \cdot p\cdot q \cdot N}{e^2(N-1) + Z_0^2 \cdot p\cdot q}$$